work on proxy pattern

realsum.bpl
@@ -1,30 +1,30 @@
 type Ref;
-var packedSumOK: [Ref] bool;
-var fracSumOK: [Ref] real;
-var packedSumGreater0: [Ref] bool;
-var fracSumGreater0: [Ref] real;
+var packedSumOKRealSum: [Ref] bool;
+var fracSumOKRealSum: [Ref] real;
+var packedSumGreater0RealSum: [Ref] bool;
+var fracSumGreater0RealSum: [Ref] real;
 
 const null: Ref;
 
 var n: [Ref]int;
 var sum: [Ref]real;
 
-procedure PackSumOK(s1:real, n1:int, this:Ref);
-requires (packedSumOK[this] == false);
+procedure PackSumOKRealSum(s1:real, n1:int, this:Ref);
+requires (packedSumOKRealSum[this] == false);
 requires (sum[this] == s1) && (n[this]==n1) &&
 	( s1 == n1 * (n1+1) / 2 );
 
-procedure UnpackSumOK(s1:real, n1:int, this:Ref);
-requires packedSumOK[this];
+procedure UnpackSumOKRealSum(s1:real, n1:int, this:Ref);
+requires packedSumOKRealSum[this];
 ensures (sum[this] == s1) && (n[this]==n1) &&
 	( s1 == n1 * (n1+1) / 2 );
 
-procedure PackSumGreater0(s1:real, this:Ref);
-requires (packedSumGreater0[this] == false);
+procedure PackSumGreater0RealSum(s1:real, this:Ref);
+requires (packedSumGreater0RealSum[this] == false);
 requires (sum[this] == s1) && (s1 > 0.0);
 
-procedure UnpackSumGreater0(s1:real, this:Ref);
-requires packedSumGreater0[this];
+procedure UnpackSumGreater0RealSum(s1:real, this:Ref);
+requires packedSumGreater0RealSum[this];
 ensures (sum[this] == s1) && (s1 > 0.0);
 
 procedure ConstructRealSum(n1:int, this:Ref)
@@ -40,20 +40,17 @@ modifies sum;
 	sum[this] := n1 * (n1 + 1) / 2;
 }
 
-procedure calculateSum()  returns (r:real, this:Ref)
+procedure calculateSumRealSum(this:Ref)  returns (r:real)
 
 { 
 	r:= sum[this];
 }
 
-procedure sumIsOK() returns (r:bool, this:Ref) {
+procedure sumIsOKRealSum( this:Ref) returns (r:bool) {
 	r := (sum[this] == (n[this] * (n[this]+1) / 2));
 }
 
-procedure sumIsGreater0(this:Ref)  returns (r:bool)
+procedure sumIsGreater0RealSum(this:Ref)  returns (r:bool)
 {
 	r:= (sum[this] > 0.0);
 }
-
-
-
