proxysum.bpl
@@ -1,0 +1,54 @@
+var packedSumOKProxySum: [Ref] bool;
+var fracSumOKProxySum: [Ref] real;
+var packedSumGreater0ProxySum: [Ref] bool;
+var fracSumGreater0ProxySum: [Ref] real;
+
+var realSum: [Ref]Ref;
+
+procedure PackSumOKProxySum(s1:real, n1:int, this:Ref);
+requires (packedSumOKProxySum[this] == false);
+requires (sum[this] == s1) && (n[this]==n1) &&
+	( s1 == n1 * (n1+1) / 2 );
+
+procedure UnpackSumOKProxySum(s1:real, n1:int, this:Ref);
+requires packedSumOKProxySum[this];
+ensures (sum[this] == s1) && (n[this]==n1) &&
+	( s1 == n1 * (n1+1) / 2 );
+
+procedure PackSumGreater0ProxySum(s1:real, this:Ref);
+requires (packedSumGreater0ProxySum[this] == false);
+requires (sum[this] == s1) && (s1 > 0.0);
+
+procedure UnpackSumGreater0ProxySum(s1:real, this:Ref);
+requires packedSumGreater0ProxySum[this];
+ensures (sum[this] == s1) && (s1 > 0.0);
+
+procedure ConstructProxySum(n1:int, this:Ref)
+modifies n,sum;
+{
+  var temp: real;
+n[this]:=n1;
+call temp := calculateSumProxySum(this);
+}
+
+procedure calculateSumProxySum(this:Ref)  returns (r:real)
+modifies n,sum;
+{ 
+  var temp : real;
+if (realSum[this]==null) {
+	call ConstructRealSum(n[this], realSum[this]);
+}
+
+	call temp := calculateSumRealSum(realSum[this]);
+  	sum[this]:=temp;
+	r:=sum[this];
+}
+
+procedure sumIsOKProxySum(this:Ref) returns (r:bool) {
+	r := (sum[this] == (n[this] * (n[this]+1) / 2));
+}
+
+procedure sumIsGreater0ProxySum(this:Ref)  returns (r:bool)
+{
+	r:= (sum[this] > 0.0);
+}
